theories/asubst_base.v
@@ -400,15 +400,19 @@ Proof. elim: xs => /= [//|x xs IHxs] /fv_cons_inv [Hclx Hclxs]. auto. Qed.
 Lemma nclosed_xs_eq_nclosed n xs: nclosed_xs xs n ↔ nclosed xs n.
 Proof. split; eauto using Forall_to_closed_xs, closed_xs_to_Forall. Qed.
 
+Lemma inf_subst_compose x σ ξ n1 n2 n3 :
+  nclosed x n1 →
+  length σ = n1 → nclosed_σ σ n2 →
+  nclosed_sub n2 n3 ξ →
+  x.|[to_subst σ.|[ξ]] = x.|[to_subst σ].|[ξ].
+Proof. intros Hclx <- Hclσ Hclξ; asimpl. apply Hclx, to_subst_compose. Qed.
+
 Lemma subst_compose x σ ξ n1 n2 n3:
   nclosed x n1 →
   length σ = n1 → nclosed_σ σ n2 →
   length ξ = n2 → nclosed_σ ξ n3 →
   x.|[to_subst σ.|[to_subst ξ]] = x.|[to_subst σ].|[to_subst ξ].
-Proof.
-  intros Hclx ? Hclσ ? Hclξ; subst; asimpl.
-  apply Hclx, to_subst_compose.
-Qed.
+Proof. intros; subst; eapply inf_subst_compose; eauto. Qed.
 
 Lemma subst_compose_idsσ x n m ξ:
   nclosed x n →
